---
layout: default
title: "Understanding the Quadratic Formula"
date: 2024-01-17
categories: math
---

Welcome to my blog post about the quadratic formula! Today, we'll explore how this formula is derived and some of its applications.

The quadratic formula is used to find the roots of a quadratic equation. A quadratic equation is any equation in the form of:

$$ ax^2 + bx + c = 0 $$

where \( a \), \( b \), and \( c \) are constants, and \( a \neq 0 \).

The roots of the quadratic equation can be found using the quadratic formula:

$$ x = \frac{-b \pm \sqrt{b^2 - 4ac}}{2a} $$

This formula is derived from completing the square in a quadratic equation.

### Example

Let's apply the quadratic formula to an example equation:

$$ 2x^2 - 4x - 6 = 0 $$

Here, \( a = 2 \), \( b = -4 \), and \( c = -6 \). Plugging these into the quadratic formula gives us:

$$ x = \frac{-(-4) \pm \sqrt{(-4)^2 - 4 \times 2 \times (-6)}}{2 \times 2} $$

$$ x = \frac{4 \pm \sqrt{16 + 48}}{4} $$

$$ x = \frac{4 \pm \sqrt{64}}{4} $$

$$ x = \frac{4 \pm 8}{4} $$

So, the solutions are \( x = 3 \) and \( x = -1 \).

I hope this post helped you understand the quadratic formula a bit better!

Remember, MathJax allows us to display complex mathematical expressions neatly in our blog posts.
